more

thys/Untyped_Lambda_Calculus/ILC_Renaming_Equivalence.thy
@@ -8,45 +8,9 @@ begin
 (* INSTANTIATING THE ABSTRACT SETTING: *)
 
 (* *)
-
-(* Error in Mazza: just using supervariables, we would 
-not be able to prove the predicate transitive: 
 inductive reneqv where
  iVar: "super xs \<Longrightarrow> {x,x'} \<subseteq> dsset xs \<Longrightarrow> reneqv (iVar x) (iVar x')"
 |iLam: "super xs \<Longrightarrow> reneqv e e' \<Longrightarrow> reneqv (iLam xs e) (iLam xs e')"
-|iApp: 
-"reneqv e1 e1' \<Longrightarrow>
- (\<forall>e e'. {e,e'} \<subseteq> sset es2 \<union> sset es2' \<longrightarrow> reneqv e e') 
- \<Longrightarrow>
- reneqv (iApp e1 es2) (iApp e1' es2')"
-*)
-
-(* The fix is to consider the equivariance closure of super, 
-which allows any permutation of the variables in a supervariable: *)
-
-definition ssuper where 
-"ssuper xs \<equiv> 
- \<exists>f. bij f \<and> |supp f| <o |UNIV::ivar set| \<and> super (dsmap f xs)"
-
-lemma super_ssuper: 
-"super xs \<Longrightarrow> ssuper xs"
-unfolding ssuper_def apply(rule exI[of _ id]) by auto
-
-lemma rrename_ssuper[simp]: 
-"bij f \<Longrightarrow> |supp f| <o |UNIV::ivar set| \<Longrightarrow> ssuper xs \<Longrightarrow> 
- ssuper (dsmap f xs)"
-unfolding ssuper_def apply safe
-subgoal for g apply(rule exI[of _ "g o inv f"])
-by (simp add: comp_assoc dstream.map_comp iterm_pre.supp_comp_bound) .
-
-(* *)
-
-(* todo: revert, as this is vacuous *)
-(* I should revert to super, and should prove euivariance under bijections that 
-send supervariables to supervariables. This is enough to prove transitivity. *)
-inductive reneqv where
- iVar: "ssuper xs \<Longrightarrow> {x,x'} \<subseteq> dsset xs \<Longrightarrow> reneqv (iVar x) (iVar x')"
-|iLam: "ssuper xs \<Longrightarrow> reneqv e e' \<Longrightarrow> reneqv (iLam xs e) (iLam xs e')"
 |iApp: 
 "reneqv e1 e1' \<Longrightarrow>
  (\<forall>e e'. {e,e'} \<subseteq> sset es2 \<union> sset es2' \<longrightarrow> reneqv e e') 
@@ -77,10 +41,10 @@ definition G :: "(T \<Rightarrow> bool) \<Rightarrow> ivar set \<Rightarrow> T \
 where
 "G \<equiv> \<lambda>R B t.  
          (\<exists>xs x x'. B = {} \<and> fst t = iVar x \<and> snd t = iVar x' \<and> 
-                    ssuper xs \<and> {x,x'} \<subseteq> dsset xs) 
+                    super xs \<and> {x,x'} \<subseteq> dsset xs) 
          \<or>
          (\<exists>xs e e'. B = dsset xs \<and> fst t = iLam xs e \<and> snd t = iLam xs e' \<and> 
-                    ssuper xs \<and> R (e,e'))
+                    super xs \<and> R (e,e'))
          \<or> 
          (\<exists>e1 e1' es2 es2'. B = {} \<and> fst t = iApp e1 es2 \<and> snd t = iApp e1' es2' \<and> 
                             R (e1,e1') \<and> (\<forall>e e'. {e,e'} \<subseteq> sset es2 \<union> sset es2' \<longrightarrow> R (e,e')))"
@@ -88,18 +52,25 @@ where
 
 (* VERIFYING THE HYPOTHESES FOR BARENDREGT-ENHANCED INDUCTION: *)
 
-lemma G_mono: "R \<le> R' \<Longrightarrow> small B \<Longrightarrow> G R B t \<Longrightarrow> G R' B t"
+lemma G_mmono: "R \<le> R' \<Longrightarrow> small B \<Longrightarrow> G R B t \<Longrightarrow> G R' B t"
 unfolding G_def by fastforce
 
 
+definition wfBij where "wfBij \<sigma> \<equiv> \<forall>xs. super xs \<longleftrightarrow> super (dsmap \<sigma> xs)"
+(* we defined closedness looking at the possible values of B in G: *)
+definition closed where "closed X \<equiv> X = {} \<or> (\<exists>xs. super xs \<and> X = dsset xs)"
+(* no need for this more elaborate setting: *)
+(* \<forall>xs. super xs \<and> dsset xs \<inter> X \<noteq> {} \<longrightarrow> dsset xs \<subseteq> X *)
+
+
 (* NB: Everything is passed \<sigma>-renamed as witnesses to exI *)
-lemma G_equiv: "ssbij \<sigma> \<Longrightarrow> small B \<Longrightarrow> G R B t \<Longrightarrow> G (\<lambda>t'. R (Tmap (inv \<sigma>) t')) (image \<sigma> B) (Tmap \<sigma> t)"
+lemma G_eequiv: "ssbij \<sigma> \<Longrightarrow> wfBij \<sigma> \<Longrightarrow> small B \<Longrightarrow> G R B t \<Longrightarrow> G (\<lambda>t'. R (Tmap (inv \<sigma>) t')) (image \<sigma> B) (Tmap \<sigma> t)"
 unfolding G_def apply(elim disjE)
   subgoal apply(rule disjI3_1)
   subgoal apply(elim exE) subgoal for xs x x'
   apply(rule exI[of _ "dsmap \<sigma> xs"]) 
   apply(rule exI[of _ "\<sigma> x"]) apply(rule exI[of _ "\<sigma> x'"]) 
-  apply(cases t) unfolding ssbij_def small_def Tmap_def 
+  apply(cases t) unfolding ssbij_def small_def Tmap_def wfBij_def
   by simp . .
   (* *)
   subgoal apply(rule disjI3_2)
@@ -107,7 +78,7 @@ unfolding G_def apply(elim disjE)
   apply(rule exI[of _ "dsmap \<sigma> xs"]) 
   apply(rule exI[of _ "rrename \<sigma> e"]) 
   apply(rule exI[of _ "rrename \<sigma> e'"])  
-  apply(cases t) unfolding ssbij_def small_def Tmap_def 
+  apply(cases t) unfolding ssbij_def small_def Tmap_def wfBij_def
   by (simp add: iterm.rrename_comps) . . 
   (* *)
   subgoal apply(rule disjI3_3)
@@ -121,9 +92,77 @@ unfolding G_def apply(elim disjE)
 lemma Tvars_dsset: "(Tfvars t - dsset xs) \<inter> dsset xs = {}" "|Tfvars t - dsset xs| <o |UNIV::ivar set|"
 apply auto by (meson card_of_minus_bound small_Tfvars small_def)
 
-lemma G_refresh: 
-"(\<forall>\<sigma> t. ssbij \<sigma> \<and> R t \<longrightarrow> R (Tmap \<sigma> t)) \<Longrightarrow> small B \<Longrightarrow> G R B t \<Longrightarrow> 
+(* *)
+
+lemma G_closed: "G R B t \<Longrightarrow> closed B"
+unfolding G_def closed_def by auto 
+
+lemma wfBij_id[simp,intro]: "wfBij id" unfolding wfBij_def by simp
+
+lemma wfBij_comp[simp]: "ssbij \<sigma> \<Longrightarrow> wfBij \<sigma> \<Longrightarrow> ssbij \<tau> \<Longrightarrow> wfBij \<tau> \<Longrightarrow> wfBij (\<tau> o \<sigma>)"
+unfolding wfBij_def by (metis ssbij_def dstream.map_comp)
+
+lemma wfBij_inv[simp]: "ssbij \<sigma> \<Longrightarrow> wfBij \<sigma> \<Longrightarrow> wfBij (inv \<sigma>)"
+unfolding wfBij_def ssbij_def 
+by (metis bij_imp_bij_inv dstream.map_comp dstream.map_id inv_inv_eq inv_o_simp1 supp_inv_bound)
+
+lemma dsset_dsmap_inv_NE: "bij \<sigma> \<Longrightarrow> dsset xs \<inter> \<sigma> ` A \<noteq> {} \<longleftrightarrow> dsset (dsmap (inv \<sigma>) xs) \<inter> A \<noteq> {}"
+by (metis bij_betw_def bij_imp_bij_betw bij_imp_bij_inv dsset_dsmap image_Int_empty inf_commute)
+
+lemma closed_wfBij: "ssbij \<sigma> \<Longrightarrow> wfBij \<sigma> \<Longrightarrow> closed A \<Longrightarrow> closed (\<sigma> ` A)"
+unfolding closed_def apply clarify  
+by (metis ILC2.ssbij_def dstream.set_map wfBij_def)
+(*
+  subgoal for xs x  apply(subst image_in_bij_eq)
+    subgoal unfolding ssbij_def by simp
+    subgoal apply(frule wfBij_inv)
+      subgoal by simp
+      subgoal apply(subst (asm) dsset_dsmap_inv_NE)
+        subgoal unfolding ssbij_def by simp
+        subgoal by (metis ILC2.ssbij_def IntD2 bij_bij_betw_inv dstream.set_map inf.absorb1 
+                    rev_image_eqI supp_inv_bound wfBij_def) . . . . 
+*)
+
+(* *)
+lemma small_ssbij_closed: 
+assumes s: "small A" "small B" "small A'" "A \<inter> A' = {}" and c: "closed A" 
+shows "\<exists>\<rho>. ssbij \<rho> \<and> wfBij \<rho> \<and> \<rho> ` A \<inter> B = {} \<and> (\<forall>a\<in>A'. \<rho> a = a)" 
+using c unfolding closed_def proof(elim disjE exE conjE)
+  assume A: "A = {}"
+  show ?thesis apply(rule exI[of _ id]) unfolding A ssbij_def by auto
+next
+  fix xs assume xs: "super xs" and A: "A = dsset xs"
+  obtain xs' where xs': "super xs'" and xss': "xs \<noteq> xs'"
+  using xs super_infinite by (smt (verit, del_insts) Collect_cong Collect_conv_if finite.simps)
+  hence ds: "dsset xs \<inter> dsset xs' = {}" using super_disj xs by auto
+  show ?thesis
+  sorry
+qed
+  
+
+
+thm refresh
+lemma refresh_super: 
+assumes V: "V \<inter> dsset xs = {}" "|V| <o |UNIV::ivar set|" "super xs"  
+shows "\<exists>f xs'. bij (f::ivar\<Rightarrow>ivar) \<and> |supp f| <o |UNIV::ivar set| \<and> 
+               dsset xs' \<inter> dsset xs = {} \<and> dsset xs' \<inter> V = {} \<and>
+               dsmap f xs = xs' \<and> id_on V f \<and> (\<forall>ys. super ys \<longleftrightarrow> super (dsmap f ys))"
+proof-
+  define A A' B where A: "A \<equiv> dsset xs" and A': "A' = V" and B: "B \<equiv> V \<union> dsset xs"
+  have 0: "small A" "small B" "small A'" "A \<inter> A' = {}" "closed A"
+  unfolding A A' B closed_def using V 
+  apply auto 
+  using small_Un small_def apply blast
+  using small_def super_disj by fastforce+
+  show ?thesis using small_ssbij_closed[OF 0] 
+  apply safe subgoal for f apply(intro exI[of _ f] exI[of _ "dsmap f xs"]) 
+  unfolding ssbij_def wfBij_def A A' B id_on_def by auto .
+qed
+
+lemma G_rrefresh: 
+"(\<forall>\<sigma> t. ssbij \<sigma> \<and> wfBij \<sigma> \<and> R t \<longrightarrow> R (Tmap \<sigma> t)) \<Longrightarrow> small B \<Longrightarrow> G R B t \<Longrightarrow> 
  \<exists>C. small C \<and> C \<inter> Tfvars t = {} \<and> G R C t"
+apply(frule G_closed)
 unfolding G_def Tmap_def apply safe
   subgoal for xs x x'
   apply(rule exI[of _ "{}"])  
@@ -137,7 +176,7 @@ unfolding G_def Tmap_def apply safe
     apply(cases t) apply simp . .
   (* *)
   subgoal for xs e e'
-  using refresh[OF Tvars_dsset, of xs t]  apply safe
+  apply(frule refresh_super[OF Tvars_dsset, of xs t]) apply safe
   subgoal for f
   apply(rule exI[of _ "f ` (dsset xs)"])  
   apply(intro conjI)
@@ -154,7 +193,7 @@ unfolding G_def Tmap_def apply safe
         subgoal unfolding ssbij_def by auto
         subgoal by (smt (verit, best) Diff_iff Un_iff iLam_rrename id_on_def 
            rrename_eq_itvsubst_iVar) . 
-        subgoal unfolding id_on_def ssbij_def by auto . . .
+        subgoal unfolding id_on_def ssbij_def wfBij_def by auto . . .
   (* *)
   subgoal for e1 e1' es2 es2'
   apply(rule exI[of _ "{}"])  
@@ -169,12 +208,14 @@ unfolding G_def Tmap_def apply safe
     apply(cases t) by simp . . 
  
 
-(* FINALLY, INTERPRETING THE Induct LOCALE: *)
+(* FINALLY, INTERPRETING THE IInduct LOCALE: *)
 
-interpretation Reneqv : Induct where dummy = "undefined :: ivar" and 
-Tmap = Tmap and Tfvars = Tfvars and G = G
+interpretation Reneqv : IInduct where dummy = "undefined :: ivar" and 
+Tmap = Tmap and Tfvars = Tfvars and G = G and closed = closed and wfBij = wfBij 
 apply standard 
-  using G_mono G_equiv G_refresh by auto
+  using G_mmono G_eequiv 
+  G_closed wfBij_id wfBij_comp wfBij_inv closed_wfBij small_ssbij_closed
+  G_rrefresh by auto  
 
 (* *)
 
@@ -205,7 +246,7 @@ corollary BE_induct_reneqv:
 assumes par: "\<And>p. small (Pfvars p)"
 and st: "reneqv t1 t2"  
 and iVar: "\<And>xs x x' p. 
-  ssuper xs \<Longrightarrow> {x,x'} \<subseteq> dsset xs \<Longrightarrow>
+  super xs \<Longrightarrow> {x,x'} \<subseteq> dsset xs \<Longrightarrow>
   R p (iVar x) (iVar x')"
 and iLam: "\<And>e e' xs p. 
   dsset xs \<inter> Pfvars p = {} \<Longrightarrow> 
